### Question:
Evaluate the infinite series $1 - \dfrac{1}{2} + \dfrac{1}{4} - \dfrac{1}{8} + \dfrac{1}{16} - ...$.

### Answer:
The infinite series can be rewritten as two sums:
$$(1 + \dfrac{1}{4} + \dfrac{1}{16} + ...) - (\dfrac{1}{2} + \dfrac{1}{8} + \dfrac{1}{32} + ...)$$
By multiplying the second sum by $\dfrac{2}{2}$, we can rewrite it as:
$$(1 + \dfrac{1}{4} + \dfrac{1}{16} + ...) - \dfrac{1}{2}(1 + \dfrac{1}{4} + \dfrac{1}{16} + ...) = $$
$$\dfrac{1}{2}(1 + \dfrac{1}{4} + \dfrac{1}{16} + ...).$$
This is an infinite decresing geometric series.
$$\dfrac{1}{2}(1 + \dfrac{1}{4} + \dfrac{1}{16} + ...) = \dfrac{1}{2}\sum_{k=0}^{\infty} (\dfrac{1}{4})^k $$
$$\dfrac{1}{2}\sum_{k=0}^{\infty} (\dfrac{1}{4})^k = \dfrac{1}{2}\dfrac{1}{1-\dfrac{1}{4}}$$
$$\dfrac{1}{2}\dfrac{1}{1-\dfrac{1}{4}} = \dfrac{1}{2}.\dfrac{4}{3}$$
$$\dfrac{1}{2}.\dfrac{4}{3} = \dfrac{2}{3}$$